examples/LinkedListSearch.bpl
@@ -1,7 +1,11 @@
+// Example inspired by: 1st Verified Software Competition (https://sites.google.com/a/vscomp.org), problem III
+
+// Run "boogaloo LinkedListSearch.bpl" to observe a possible execution (use axioms and assumptions to constrain possible executions)
+
 // Reference type
 type ref;
 
-// null-reference
+// Null-reference
 const null: ref;
 
 // Maps a list node to the stored value  
@@ -15,9 +19,7 @@ const head: ref;
 
 // Is list starting at "node" acyclic?
 function acyclic(node: ref): bool
-{
-  node == null || (index[node] < index[next[node]] && acyclic(next[node]))
-}
+{ node == null || (index[node] < index[next[node]] && acyclic(next[node])) }
 
 // How many times "next" should be applied to reach "node'" starting from "node"?
 function distance(node, node': ref): int
@@ -69,8 +71,5 @@ axiom (forall i, j: int :: 0 <= i && i < j && j < N ==> at(head, i) != at(head, 
 
 procedure Main() returns (result: int)
 {
-  // assume acyclic(head);
-  // assume length(head) == N;
-  // assume (forall i, j: int :: 0 <= i && i < j && j < N ==> at(head, i) != at(head, j));
   call result := search(0);
 }
