examples/McCarthy-91.bpl
@@ -1,5 +1,6 @@
 // Original example from: https://boogie.codeplex.com/ Test/textbook
 
+// Run "boogaloo -p F McCarthy-91.bpl" to observe a possible execution
 // Run "boogaloo test -p F McCarthy-91.bpl" to test F exhaustively within the default range of inputs
 // Run "boogaloo rtest -p F McCarthy-91.bpl" to test F on a default number of random inputs
 
